theories/All.v
@@ -1,0 +1,4 @@
+From Tableaux Require Export Prelude.
+From Tableaux Require Export Proofs.
+From Tableaux Require Export Skolemization.
+From Tableaux Require Export Syntax.
