theories/Skolemization.v
@@ -1,0 +1,28 @@
+(** * Skolemization: a generic class for Skolemization *)
+
+From Tableaux Require Import Prelude.
+From Tableaux Require Import Syntax.
+
+(** In this file, we implement first-order Skolemization in the framework of Cantone
+    and Nicolosi-Asmundo (in their paper _A Sound Framework for δ-Rule Variants
+    in Free-Variable Semantic Tableaux_). The goal is to be able to be
+    Skolemization-independent in the definition of tableaux and make it work seamlessly
+    for different instances of this class. *)
+Section SkolemizationDef.
+  Context (pred func var : Atom).
+
+  #[local] Definition set_var := set_atom var.
+  #[local] Definition set_func := set_atom func.
+
+  Class Skolemization_ :=
+    { sko :> Form_ pred func var -> set_var -> set_func -> Term_ func var
+    ; symbol : Form_ pred func var -> set_var -> set_func -> func
+
+    ; symbol_is_sko : forall F S Sf, get_symbol (sko F S Sf) = Some (symbol F S Sf) }.
+End SkolemizationDef.
+
+Arguments sko {_ _ _} _ _ _.
+Arguments symbol {_ _ _} _ _ _.
+Arguments symbol_is_sko {_ _ _} _ _ _.
+
+Definition Skolemization := Skolemization_ string string nat.
